add ReadNoOp step

disk-betree/BlockCache.dfy
@@ -5,6 +5,7 @@ include "Graph.dfy"
 include "Disk.dfy"
 
 module LBAType {
+
   import NativeTypes
 
   type LBA(==,!new) = NativeTypes.uint64
@@ -67,12 +68,11 @@ abstract module BlockCache refines Transactable {
   datatype Step =
     | WriteBackStep(ref: Reference)
     | WriteBackSuperblockStep
-    //| DirtyStep(ref: Reference, block: Node)
-    //| AllocStep(ref: Reference, block: Node)
     | UnallocStep(ref: Reference)
     | PageInStep(ref: Reference)
     | PageInSuperblockStep
     | EvictStep(ref: Reference)
+    | ReadNoOpStep
     | TransactionStep(ops: seq<Op>)
 
   predicate WFPersistentSuperblock(superblock: Superblock)
@@ -248,6 +248,12 @@ abstract module BlockCache refines Transactable {
     && s' == s.(cache := MapRemove(s.cache, {ref}))
   }
 
+  predicate ReadNoOp(k: Constants, s: Variables, s': Variables, dop: DiskOp)
+  {
+    && dop.ReadOp?
+    && s' == s
+  }
+
   predicate Init(k: Constants, s: Variables)
   {
     s == Unready
@@ -261,9 +267,7 @@ abstract module BlockCache refines Transactable {
       case PageInStep(ref) => PageIn(k, s, s', dop, ref)
       case PageInSuperblockStep => PageInSuperblock(k, s, s', dop)
       case EvictStep(ref) => Evict(k, s, s', dop, ref)
-
-      //case DirtyStep(ref, block) => Dirty(k, s, s', dop, ref, block)
-      //case AllocStep(ref, block) => Alloc(k, s, s', dop, ref, block)
+      case ReadNoOpStep => ReadNoOp(k, s, s', dop)
       case TransactionStep(ops) => Transaction(k, s, s', dop, ops)
     }
   }
@@ -443,9 +447,7 @@ abstract module BlockCache refines Transactable {
       case PageInStep(ref) => PageInStepPreservesInvariant(k, s, s', dop, ref);
       case PageInSuperblockStep => PageInSuperblockStepPreservesInvariant(k, s, s', dop);
       case EvictStep(ref) => EvictStepPreservesInvariant(k, s, s', dop, ref);
-
-      //case DirtyStep(ref, block) => DirtyStepPreservesInvariant(k, s, s', dop, ref, block);
-      //case AllocStep(ref, block) => AllocStepPreservesInvariant(k, s, s', dop, ref, block);
+      case ReadNoOpStep => { }
       case TransactionStep(ops) => TransactionStepPreservesInvariant(k, s, s', dop, ops);
     }
   }
